# The Number and Vector Parts of a Quaternion

Let

$$q=a+bi+cj+dk=a+p$$

![](a8963b60615cc06d0e15430fabd69439_MD5.jpeg)

Consider the vector

$$p_1=b_1i+c_1j+d_1k, \quad p_2=b_2i+c_2j+d_2k$$

So that their product

$$
\begin{equation}
 \begin{split}
  p_1p_2=&-(b_1b_2+c_1c_2+d_1d_2)\\
  &+(c_1d_2-d_1c_2)i+(d_1b_2-b_1d_2)j+(b_1c_2-c_1b_2)k
 \end{split}\tag{1}
\end{equation}
$$

^975c41

#Math/ComplexNumber/QuaternionProduct

# Scalar Product of Vectors

$$
\begin{aligned}
(p_1, p_2)&\coloneqq\left|p_1\right|\left|p_2\right|\cos\varphi\\
&=b_1b_2+c_1c_2+d_1d_2
\end{aligned}
$$

# Cross Product of Vectors

$$
\begin{aligned}
 \left[ p_1, p_2\right]&\coloneqq(c_1d_2-d_1c_2)i+(d_1b_2-b_1d_2)j+(b_1c_2-c_1b_2)k\\
 &=|p_1||p_2|\sin\varphi \cdot e_{\left[ p_1, p_2\right]}
\end{aligned}
$$

$$\therefore p_1p_2=-(p_1, p_2)+[p_1, p_2]$$

# The Geometric Interpretation of the Multiplication of a Quaternion by a Pure Vector Quaternion

Let

$$q=a+bi+cj+dk$$

be a unit quaternion (whose absolute value is $1$). Then

$$\begin{gathered}
a^2+b^2+c^2+d^2=1\\
q=a+q^{\prime}
\end{gathered}$$

where $q'$ is the vector $bi+cj+dk$. Since $|a^2|+|q^{\prime}|^2=1$, there exists an angle $\varphi$, such that

$$a=\cos\varphi, \quad|q^{\prime}|=\sin\varphi.$$

Clearly, $q^{\prime}=|q^{\prime}|\textit{ p}$, where $p$ is a vector of unit length. Hence

$$q=\cos\varphi+p\sin\varphi$$

Suppose a vector $v$ that is _perpendicular_ to $p$ but otherwise arbitrary. We have

$$
\begin{aligned}
qv&=(\cos\varphi+p\sin\varphi)v\\
&=v\cos\varphi+pv\sin\varphi\\
&=v\cos\varphi+\{-(p, v)+[p, v]\}\sin\varphi\end{aligned}
$$

Since $q$ and $v$ are perpendicular, $(p, v)$ is zero and $[p, v]$ is a vector of length $|p|\cdot|v|\cdot\sin\frac\pi2=|v|$. Denote this vector by $pv=\tilde{v}$ , we have

$$qv=v\cos\varphi+\tilde{v}\sin\varphi $$

Thus, if $p$ is a vector of length $1$ and $v$ is any vector perpendicular to $p$, then by multiplying $v$ on the left by the quaternion $q=\cos \varphi+p\sin\varphi$ we rotate it about $p$ through the angle $\varphi$.

![](14dc82f7d934d782344be78b79865e5b_MD5.jpeg)

# Representation of an Arbitrary Rotation in Space by Means of Quaternions

Consider an _arbitrary_ vector $v$ and the more complex expression

$$qvq^{-1}$$

First it is easy to see that

$$q^{-1}=\cos\varphi-p\sin\varphi$$

In fact, $(\cos\varphi+p\sin\varphi)(\cos\varphi-p\sin\varphi)=\cos^2\varphi-p^2\sin^2\varphi=\cos^2\varphi+\sin^2\varphi=1$.

Second, from [[#^975c41|definition (1)]] we can easily derive that if $q_1$ and $q_2$ are perpendicular, then $q_1q_2=-q_2q_1$.

Note that $v$ is an arbitrary vector. We decompose it into two components, $v=v_1+v_2$, where $v_1$ is a vector perpendicular to $p$ and $v_2$ is proportional to $p$. Then

$$qvq^{-1}=qv_1q^{-1}+qv_2q^{-1}$$

## Perpendicular component

Since $v_1$ is perpendicular to $p$, then

$$
\begin{split}qv_1q^{-1}&=qv_1(\cos\varphi-p\sin\varphi)\\
&=qv_1\cos\varphi-(qv_1)p\sin\varphi\end{split}
$$

Notice that $qv_1=v_1\cos\theta+[p, v_1]\sin\theta$ is again a vector perpendicular to $p$. Hence $(qv_1)p=-p(qv_1)$. Thus

$$\begin{split}qv_1q^{-1}&=qv_1\cos\varphi+p(qv_1)\sin\varphi\\
&=qv_1\cos\varphi+\widetilde{qv_1}\sin\varphi\end{split}$$

The expression on the right is the vector obtained by rotating $qv_1$ about $p$ through the angle $\varphi$. Also, the vector $qv$ is obtained from $v$ by the same rotation. Then it is clear that $qvq^{-1}$ is the result of rotating $v$ about $p$ through the angle $2\varphi$.

## Proportional component

Since $v_2$ is proportional to $p$, which is $v_2=\lambda p$, then clearly $qv=vq$ and

$$qv_2q^{-1}=v_2qq^{-1}=v_2$$

## Conclusion

Consider an arbitrary vector $v=v_1+v_2$, then

$$qvq^{-1}=qv_1q^{-1}+qv_2q^{-1}=qv_1q^{-1}+v_2$$

We have shown that *the rotation about* $p$ *through the angle* $2\varphi$ *takes the vector* $v$ *into the vector* $qvq^{-1}$ , where

$$q=\cos\varphi+p\sin\varphi$$

# The Problem of "Composition" of Rotations

The result of successive application of two rotations corresponding to the quaternions $q_1$ and $q_2$ is the rotation corresponding to the quaternion $q_2q_1$.

$$v_2=q_2v_1q_2^{-1}=q_2(q_1vq_1^{-1})q_2^{-1}=(q_2q_1)v(q_2q_1)^{-1}$$
